Fix the Hash proofs to use new hoare framework

src/Compare.v
@@ -27,28 +27,50 @@ Proof.
   unfold compare. step. step. step.
 Qed.
 
-Definition compare_hash T sz (buf1 buf2 : word sz) hm rx : prog T :=
-  let^ (h1, hm) <- Hash buf1 hm;
-  let^ (h2, hm) <- Hash buf2 hm;
+Definition compare_hash T sz (buf1 buf2 : word sz) rx : prog T :=
+  h1 <- Hash buf1;
+  h2 <- Hash buf2;
   If (weq h1 h2) {
     rx true
   } else {
     rx false
   }.
 
+
+Lemma hash_safe_eq : forall hm h1 h2 sz (k1 k2 : word sz),
+  hash_safe hm h1 k1 ->
+  hash_safe (upd_hashmap' hm h1 k1) h2 k2 ->
+  h1 = h2 ->
+  k1 = k2.
+Proof.
+  unfold hash_safe, upd_hashmap'; intros. subst.
+  destruct (weq h2 default_hash) eqn:Hdef.
+
+  destruct hm;
+    (unfold hashmap_get in *; rewrite Hdef in *;
+    destruct H as [ H' | H' ]; inversion H';
+    destruct H0 as [ H0' | H0' ]; inversion H0';
+    rewrite H2 in H3; pose proof (eq_sigT_snd H3); autorewrite with core in *; auto).
+
+  subst.
+  rewrite upd_hashmap_eq in H0; auto.
+  destruct H0 as [ H0' | H0' ]; inversion H0'.
+  pose proof (eq_sigT_snd H1). autorewrite with core in *. auto.
+Qed.
+
 Theorem compare_hash_ok :
-  forall sz (buf1 buf2 : word sz) hm,
+  forall sz (buf1 buf2 : word sz),
   {< (_ : unit),
   PRE         emp
   POST RET:r  emp * [[ r = true -> buf1 = buf2 ]] * [[ r = false -> buf1 <> buf2 ]]
   CRASH       emp
-  >} compare_hash buf1 buf2 hm.
+  >} compare_hash buf1 buf2.
 Proof.
-  unfold compare_hash. step. step. step.
-  step. rewrite H5 in H7. rewrite H7 in H8.
-  pose proof (eq_sigT_snd H8).
-  autorewrite with core in *. auto.
-  step.
+  unfold compare_hash.
+  hoare.
+
+  rewrite <- H5 in H9.
+  eapply hash_safe_eq; eauto.
 
   Grab Existential Variables.
   all: eauto.
